Added corresponence lemmas for the generalised word array abstractions
Lemmas for showing correspondence between the update and value semantic
abstractions, vval_typing and uval_typing_frame were added for the word
array functions wordarray_length, wordarray_get and wordarray_put2.
These lemmas were added since they are now more general than the
previous versions, i.e. will hold for standard word sizes, and hence
can be easily used in automation to prove the various assumptions
which are maded when showing correspondence between the shallow and C.

cogent/examples/wa_connect/WordArray_Abstractions.thy
@@ -44,6 +44,13 @@ fun size_of_num_type :: "num_type \<Rightarrow> ptrtyp"
 "size_of_num_type U32 = 4" |
 "size_of_num_type U64 = 8"
 
+fun zero_num_lit :: "num_type \<Rightarrow> lit"
+  where
+"zero_num_lit U8 = LU8 0" |
+"zero_num_lit U16 = LU16 0" |
+"zero_num_lit U32 = LU32 0" |
+"zero_num_lit U64 = LU64 0"
+
 
 section "WordArray Locale Definition"
 locale WordArray = main_pp_inferred begin
@@ -73,7 +80,7 @@ locale WordArray = main_pp_inferred begin
     (case au of
       UWA (TPrim (Num t)) len arr \<Rightarrow>
         (case av of 
-          VWA (TPrim (Num t)) xs \<Rightarrow> unat len = length xs \<and> 
+          VWA (TPrim (Num t)) xs \<Rightarrow> unat len = length xs \<and> \<tau>s = [TPrim (Num t)] \<and>
           (\<forall>i < len. \<exists>x. \<sigma> (arr + size_of_num_type t * i) = option.Some (UPrim x) \<and> xs ! unat i = VPrim x \<and> lit_type x = Num t)
           | _ \<Rightarrow> False)
       | _ \<Rightarrow> (case av of
@@ -263,11 +270,11 @@ definition upd_wa_get_0
   "upd_wa_get_0 x y =
       (let (x1, x2) = x;
            (y1, y2) = y
-      in x1 = y1 \<and> (\<exists>p idx t len arr v. x2 = URecord [
+      in x1 = y1 \<and> (\<exists>p idx t len arr. x2 = URecord [
           (UPtr p (RCon ''WordArray'' [RPrim (Num t)]), RPtr (RCon ''WordArray'' [RPrim (Num t)])),
           (UPrim (LU32 idx), RPrim (Num U32))] \<and> x1 p = option.Some (UAbstract (UWA (TPrim (Num t)) len arr)) \<and>
-          y2 = UPrim v \<and> lit_type v = Num t \<and> (idx < len \<longrightarrow> x1 (arr + size_of_num_type t * idx) = option.Some y2) \<and>
-            (\<not> idx < len \<longrightarrow> (v = LU8 0 \<or> v = LU16 0 \<or> v = LU32 0 \<or> v = LU64 0))))"
+          (idx < len \<longrightarrow> x1 (arr + size_of_num_type t * idx) = option.Some y2) \<and>
+            (\<not> idx < len \<longrightarrow> y2 = UPrim (zero_num_lit t))))"
 
 definition upd_wa_length_0
   where
@@ -292,21 +299,21 @@ subsubsection "Value Semantics"
     or we modify the current type to include the word type. \<close>
 definition val_wa_length
   where
-  "val_wa_length x y = (\<exists>xs len ts. x = VAbstract (VWA (TPrim (Num ts)) xs) \<and> y = VPrim (LU32 len) \<and> 
+  "val_wa_length x y = (\<exists>xs len t. x = VAbstract (VWA (TPrim (Num t)) xs) \<and> y = VPrim (LU32 len) \<and> 
                           length xs = unat len)" 
 
 definition val_wa_get
   where
   "val_wa_get x y =
-      (\<exists>xs ts idx v. x = VRecord [VAbstract (VWA (TPrim (Num ts)) xs), VPrim (LU32 idx)] \<and>
-       y = VPrim v \<and> lit_type v = Num ts \<and> (unat idx < length xs \<longrightarrow> xs ! unat idx = y) \<and> 
-       (\<not> unat idx < length xs \<longrightarrow> (v = LU8 0 \<or> v = LU16 0 \<or> v = LU32 0 \<or> v = LU64 0)))" 
+      (\<exists>xs t idx v. x = VRecord [VAbstract (VWA (TPrim (Num t)) xs), VPrim (LU32 idx)] \<and>
+       y = VPrim v \<and> lit_type v = Num t \<and> (unat idx < length xs \<longrightarrow> xs ! unat idx = y) \<and> 
+       (\<not> unat idx < length xs \<longrightarrow> zero_num_lit t = v))" 
 
 definition val_wa_put2
   where
   "val_wa_put2 x y =
-      (\<exists>xs ts idx val. x = VRecord [VAbstract (VWA (TPrim (Num ts)) xs), VPrim (LU32 idx), VPrim val] \<and>
-       lit_type val = Num ts \<and> y = VAbstract (VWA (TPrim (Num ts)) (xs[unat idx := VPrim val])))" 
+      (\<exists>xs t idx val. x = VRecord [VAbstract (VWA (TPrim (Num t)) xs), VPrim (LU32 idx), VPrim val] \<and>
+       lit_type val = Num t \<and> y = VAbstract (VWA (TPrim (Num t)) (xs[unat idx := VPrim val])))" 
 
 
 fun \<xi>m :: "(char list, vatyp) vabsfuns" 
@@ -333,48 +340,13 @@ subsection "Level 1 \<xi> Abstractions"
     levels are introduced, i.e. when third, fourth ... calls are introduced, these abstractions
     should probably be automatically generated. \<close>
 
-(*
-function \<xi>1 :: "(char list, atyp, 32 word) uabsfuns" 
-  and upd_wa_foldnb_0  :: "(char list, atyp, 32 word) ufundef" 
-(*  and upd_wa_mapnb_0  :: "(char list, atyp, 32 word) ufundef" *)
-  where
-  "\<xi>1 x y z = 
-    (if x = ''wordarray_fold_no_break_0'' then upd_wa_foldnb_0 y z
-     else (if x = ''wordarray_map_no_break_0'' then False 
-           else \<xi>0 x y z))" 
-| "upd_wa_foldnb_0 (b1, b2) c = (\<exists>p frm to f ts acc len arr.
-    b2 = URecord [(UPtr p (RCon ''WordArray'' [RPrim (Num U32)]), RPtr (RCon ''WordArray'' [RPrim (Num U32)])),
-      (UPrim (LU32 frm), RPrim (Num U32)), (UPrim (LU32 to), RPrim (Num U32)),
-      (UFunction f ts, RFun), (UPrim (LU32 acc), RPrim (Num U32)), (UUnit, RUnit)] \<and> 
-    b1 p = option.Some (UAbstract (WAU32 len arr)) \<and>
-    (if frm < min to len 
-      then (\<exists>v b1' acc'. (b1 (arr + 4 * frm) = option.Some (UPrim (LU32 v))) \<and> 
-        (\<xi>1, [(URecord [(UPrim (LU32 v), RPrim (Num U32)), (UPrim (LU32 acc), RPrim (Num U32)), 
-          (UUnit, RUnit)])] \<turnstile> (b1, App (Fun f ts) (Var 0)) \<Down>! (b1', UPrim (LU32 acc'))) \<and>
-        upd_wa_foldnb_0 (b1', URecord [(UPtr p (RCon ''WordArray'' [RPrim (Num U32)]), RPtr (RCon ''WordArray'' [RPrim (Num U32)])),
-          (UPrim (LU32 (frm + 1)), RPrim (Num U32)), (UPrim (LU32 to), RPrim (Num U32)),
-          (UFunction f ts, RFun), (UPrim (LU32 acc'), RPrim (Num U32)), (UUnit, RUnit)]) c)
-    else (b1, b2) = c))"
-  by pat_completeness auto
-
-termination \<xi>1
-  apply (relation "measure 
-    (\<lambda>x. case x of Inl (_, _, _) \<Rightarrow> Suc (unat ((max_word :: 32 word)))
-             | Inr ((a1, a2), _) \<Rightarrow> 
-                      (case a2 of URecord [] \<Rightarrow> 0
-                                        | _ \<Rightarrow> 0))")
-     apply clarsimp
-  apply clarsimp
-  sorry
-*)
-
 subsubsection "Update Semantics"
 
 type_synonym ('f, 'a, 'l) ufoldmapdef = "(char list, atyp, 32 word) uabsfuns \<Rightarrow> ('f, 'a, 'l) store \<Rightarrow> 
                                          32 word \<Rightarrow> 32 word \<Rightarrow> 32 word \<Rightarrow>
                                         'f expr \<Rightarrow> ('f, 'a, 'l) uval \<Rightarrow> ('f, 'a, 'l) uval \<times> ptrtyp set\<Rightarrow>
                                         (('f, 'a, 'l) store \<times> ('f, 'a, 'l) uval) \<Rightarrow> bool"
-
+(*
 function upd_wa_mapnb_bod_0 :: "(char list, atyp, 32 word) ufoldmapdef"
   where
   "upd_wa_mapnb_bod_0 \<xi>\<^sub>u \<sigma> p frm to f acc (obsv, s) res = (\<exists>t len arr. 
@@ -396,6 +368,7 @@ termination
    apply (cut_tac y = to in word_not_simps(3); clarsimp simp: word_less_nat_alt)
   apply linarith
   done
+*)
 
 function upd_wa_foldnb_bod_0 :: "(char list, atyp, 32 word) ufoldmapdef"
   where
@@ -416,7 +389,7 @@ termination
    apply (cut_tac y = to in word_not_simps(3); clarsimp simp: word_less_nat_alt)
   apply linarith
   done
-declare upd_wa_mapnb_bod_0.simps[simp del]
+
 declare upd_wa_foldnb_bod_0.simps[simp del]
 
 lemma upd_wa_foldnb_bod_0_to_geq_len:
@@ -813,7 +786,31 @@ definition upd_wa_foldnb_0  :: "(char list, atyp, 32 word) ufundef"
                                 TPrim (Num U32)) \<and>
                               upd_wa_foldnb_bod_0 \<xi>0 y1 p frm to (AFun f ts) (UPrim (LU32 acc)) (UUnit, {}) z
           | _ \<Rightarrow> False)))"
-
+\<comment>\<open> It is hard to generalise the definition for wordarray_fold because we require the type mapping
+   for functions which is only defined at compiled time \<close>
+(*
+definition upd_wa_foldnb  :: "(char list, atyp, 32 word) ufundef" 
+  where
+  "upd_wa_foldnb y z = 
+    (let (y1, y2) = y;
+         (z1, z2) = z
+      in (\<exists>p frm to acc r x t u v.
+        y2 = URecord [(UPtr p (RCon ''WordArray'' [RPrim (Num t)]), 
+                      RPtr (RCon ''WordArray'' [RPrim (Num t)])),
+                      (UPrim (LU32 frm), RPrim (Num U32)), (UPrim (LU32 to), RPrim (Num U32)),
+                      (x, RFun), (UPrim (LU32 acc), RPrim (Num U32)), (UUnit, RUnit)] \<and> 
+        y1 = z1 \<and> y1 p = z1 p \<and> (\<exists>len arr. y1 p = option.Some (UAbstract (UWA (TPrim (Num U32)) len arr)) \<and> 
+          (\<forall>i<len. y1 (arr + size_of_num_type t * i) = z1 (arr + size_of_num_type t * i))) \<and> z2 = UPrim (LU32 r) \<and>
+        (case x of
+            UFunction f ts \<Rightarrow> (\<Xi>, [], [option.Some abbreviatedType1] \<turnstile> (App (Fun f ts) (Var 0)) : 
+                                TPrim (Num U32)) \<and> 
+                              upd_wa_foldnb_bod_0 \<xi>0 y1 p frm to (Fun f ts) (UPrim (LU32 acc)) (UUnit, {}) z
+          | UAFunction f ts \<Rightarrow> (\<Xi>, [], [option.Some abbreviatedType1] \<turnstile> (App (AFun f ts) (Var 0)) : 
+                                TPrim (Num U32)) \<and>
+                              upd_wa_foldnb_bod_0 \<xi>0 y1 p frm to (AFun f ts) (UPrim (LU32 acc)) (UUnit, {}) z
+          | _ \<Rightarrow> False)))"
+*)
+(*
 definition upd_wa_mapnb_0  :: "(char list, atyp, 32 word) ufundef" 
   where
   "upd_wa_mapnb_0 y z = 
@@ -831,7 +828,7 @@ definition upd_wa_mapnb_0  :: "(char list, atyp, 32 word) ufundef"
             UFunction f ts \<Rightarrow> upd_wa_mapnb_bod_0 \<xi>0 y1 p frm to (Fun f ts) (UUnit) (UUnit, {}) z
           | UAFunction f ts \<Rightarrow> upd_wa_mapnb_bod_0 \<xi>0 y1 p frm to (AFun f ts) (UUnit) (UUnit, {}) z
           | _ \<Rightarrow> False)))"
-
+*)
 fun \<xi>1 :: "(char list, atyp, 32 word) uabsfuns" 
   where
   "\<xi>1 x y z = 
